created repo

leetcde_283_with_hax/hax_output/HaxOutput/Basic.lean
@@ -13,4 +13,25 @@ set_option linter.unusedVariables false
 def Playground._.requires (x : u8) : Result Bool := do
   (← Rust_primitives.Hax.Machine_int.lt x (16 : u8))
 
+def Playground.__1.future
+  (T : Type) (x : T)
+  : Result (Rust_primitives.Hax.Tuple2 T T)
+  := do
+  let hax_temp_output : T ← (pure x);
+  (Rust_primitives.Hax.Tuple2.mk x hax_temp_output)
+
+def Playground.__1.ensures (x : u8) (res : u8) : Result Bool := do true
+
 def Playground.square (x : u8) : Result u8 := do (← x *? x)
+
+
+theorem square_spec (x: u8) :
+  ⦃ Playground._.requires x ⦄
+  Playground.square x
+  ⦃ Playground.__1.ensures x ⦄
+:= by
+  mvcgen
+  simp [Playground._.requires, Playground.__1.ensures, Playground.square] at *
+  intros
+  rw [UInt8.HaxMul_spec_bv_rw]
+  bv_decide
